src/Language/PlutusIR/Semantics/Static/Implementations.v
@@ -2,6 +2,7 @@ Require Import PlutusCert.Language.PlutusIR.
 Import NamedTerm.
 Require Export PlutusCert.Language.PlutusIR.Semantics.Static.Map.
 Require Export PlutusCert.Language.PlutusIR.Semantics.Static.TypeSubstitution.
+Require Export PlutusCert.Language.PlutusIR.Semantics.Static.TypeSubstitution.CaptureAvoiding.
 
 Require Import Coq.Lists.List.
 Require Import Coq.Program.Basics.
@@ -383,6 +384,8 @@ Definition fromDecl (tvd : tvdecl tyname) : Context :=
     
 Definition unwrapIFix (F : Ty) (K : Kind) (T : Ty) : Ty := (Ty_App (Ty_App F (Ty_Lam "X" K (Ty_IFix F (Ty_Var "X")))) T).
 
+
+(*
 Fixpoint beta_reduce (T : Ty) : Ty :=
   match T with
   (* Beta-reduction *)
@@ -398,3 +401,36 @@ Fixpoint beta_reduce (T : Ty) : Ty :=
   | Ty_IFix F T => Ty_IFix (beta_reduce F) (beta_reduce T)
   | Ty_Builtin st => Ty_Builtin st
   end.
+*)
+
+
+Inductive normalise : Ty -> Ty -> Prop :=
+  | N_BetaReduce : forall bX K T1 T2 T',
+      substituteTCA bX T2 T1 T' ->
+      normalise (Ty_App (Ty_Lam bX K T1) T2) T'
+  | N_TyApp : forall T1 T2 T1' T2',
+      ~(exists X K T1_body, T1 = Ty_Lam X K T1_body) ->
+      normalise T1 T1' ->
+      normalise T2 T2' ->
+      normalise (Ty_App T1 T2) (Ty_App T1' T2')
+  | N_TyFun : forall T1 T2 T1' T2',
+      normalise T1 T1' ->
+      normalise T2 T2' ->
+      normalise (Ty_Fun T1 T2) (Ty_Fun T1' T2')
+  | N_TyForall : forall bX K T0 T0',
+      normalise T0 T0' ->
+      normalise (Ty_Forall bX K T0) (Ty_Forall bX K T0')
+  | N_TyLam : forall bX K T0 T0',
+      normalise T0 T0' ->
+      normalise (Ty_Lam bX K T0) (Ty_Lam bX K T0')
+  | N_TyVar : forall X,
+      normalise (Ty_Var X) (Ty_Var X)
+  | N_TyIFix : forall F T F' T',
+      normalise F F' ->
+      normalise T T' ->
+      normalise (Ty_IFix F T) (Ty_IFix F' T')
+  | N_TyBuiltin : forall st,
+      normalise (Ty_Builtin st) (Ty_Builtin st)
+  .
+
+#[export] Hint Constructors normalise : core.
