src/Language/PlutusIR/Semantics/TypeSafety/SubstitutionPreservesTyping/AnnotationSubstitution.v
@@ -2,156 +2,92 @@ Require Import PlutusCert.Language.PlutusIR.
 Import NamedTerm.
 Require Import PlutusCert.Language.PlutusIR.Semantics.Static.
 Require Import PlutusCert.Language.PlutusIR.Semantics.Dynamic.AnnotationSubstitution.
+Require Import PlutusCert.Language.PlutusIR.Semantics.TypeSafety.NormalisationPreservesKinding.
 Require Import PlutusCert.Language.PlutusIR.Semantics.TypeSafety.SubstitutionPreservesTyping.TypeSubstitution.
 
 Require Import Coq.Logic.FunctionalExtensionality.
 
-Definition tass := list (name * Ty).
+Definition upd (a : tyname) (T' : Ty ) (Gamma : partial_map Ty) :=
+  fun x =>
+    match Gamma x with
+    | None => None
+    | Datatypes.Some T => Datatypes.Some (substituteT a T' T)
+    end.
 
-Fixpoint mupdate {X:Type} (m : partial_map X) (xts : list (string * X)) :=
-  match xts with
-  | nil => m
-  | ((x, v) :: xts') => x |-> v ; (mupdate m xts')
-  end.
-  
-Fixpoint lookup {X:Type} (k : string) (l : list (name * X)) : option X :=
-  match l with
-  | nil => None
-  | (j,x) :: l' => if String.eqb j k then Datatypes.Some x else lookup k l'
-  end.
-
-Fixpoint drop {X:Type} (n:string) (nxs:list (string * X)) : list (string * X) :=
-  match nxs with
-  | nil => nil
-  | (n',x) :: nxs' => if String.eqb n' n then drop n nxs' else (n',x) :: (drop n nxs')
-  end.
-
-Inductive UpdateContext (X : tyname) (U : Ty) : tass -> tass -> Prop :=
-  | UC_nil :
-      UpdateContext X U nil nil
-  | UC_Some : forall x T T' c c',
-      UpdateContext X U c c' ->
-      substituteTCA X U T T' ->
-      UpdateContext X U ((x, T) :: c) ((x, T') :: c').
-
-Lemma UpdateContext_domains_match : forall X U c c',
-    UpdateContext X U c c' ->
-    forall x T,
-      lookup x c = Datatypes.Some T ->
-      exists T',
-        lookup x c' = Datatypes.Some T'.
+Lemma upd_empty : forall X U,
+    upd X U empty = empty.
 Proof.
-  intros X U c c' UC.
-  induction UC; intros x0 T0 C.
-  - discriminate.
-  - simpl. 
-    simpl in C.
-    destruct (x =? x0) eqn:Heqb.
-    + exists T'. auto.
-    + apply IHUC with T0.
-      auto.
+  intros X U.
+  unfold upd.
+  simpl.
+  reflexivity.
 Qed.
 
-Lemma UpdateContext_substituteTCA : forall X U c c',
-    UpdateContext X U c c' ->
-    forall x T T',
-      lookup x c = Datatypes.Some T ->
-      lookup x c' = Datatypes.Some T' ->
-      substituteTCA X U T T'.
+Lemma upd__substituteT : forall Gamma x X U T,
+    Gamma x = Datatypes.Some T ->
+    (upd X U Gamma) x = Datatypes.Some (substituteT X U T).
 Proof.
-  intros X U c c' UC.
-  induction UC; intros x' T0' T0'' E1 E2.
-  - destruct x'; discriminate.
-  - inversion E1. subst.
-    inversion E2. subst.
-    destruct (x =? x').
-    + inversion H1. subst.
-      inversion H2. subst.
-      assumption. 
-    + apply IHUC with x'; assumption.
+  intros.
+  unfold upd.
+  rewrite H.
+  reflexivity.
 Qed.
 
-Lemma mupdate_lookup : forall (c : tass) (x : name),
-    lookup x c = (mupdate empty c) x.
+Lemma upd_absorbs_substituteT : forall x X U T Gamma,
+    (x |-> (substituteT X U T); upd X U Gamma) = upd X U (x |-> T; Gamma).
 Proof.
-  induction c.
-  - intros.
-    simpl.
+  intros.
+  unfold extendT.
+  simpl.
+  f_equal.
+  apply functional_extensionality.
+  intros.
+  destruct (x =? x0) eqn:Heqb.
+  - (* x = x0 *)
+    apply eqb_eq in Heqb as Heq.
+    subst.
+    unfold upd.
+    rewrite update_eq.
+    rewrite update_eq.
     reflexivity.
-  - intros.
-    simpl.
-    destruct a.
-    destruct (s =? x) eqn:Heqb.
-    + apply eqb_eq in Heqb as Heq.
-      subst.
-      rewrite update_eq.
-      reflexivity.
-    + apply eqb_neq in Heqb as Hneq.
-      rewrite update_neq; auto.
+  - (* x <> x0 *)
+    apply eqb_neq in Heqb as Hneq.
+    unfold upd.
+    rewrite update_neq; auto.
+    rewrite update_neq; auto.
 Qed.
 
 (** ** Predicates *)
 Definition P_Term (t : Term) :=
-  forall Delta Gamma Gamma' X U c c', 
-    UpdateContext X U c c' ->
-    Gamma = mupdate empty c ->
-    Gamma' = mupdate empty c' -> 
-    forall K t' T T',
-      (X |K-> K; (Delta, Gamma)) |-+ t : T ->
-      empty |-* U : K ->
-      substituteA X U t t' ->
-      substituteTCA X U T T' ->
-      (Delta, Gamma') |-+ t' : T'.
+  forall Delta Gamma X K U T t',
+    (X |K-> K; (Delta, Gamma)) |-+ t : T ->
+    empty |-* U : K ->
+    substituteA X U t t' ->
+    (Delta, upd X U Gamma) |-+ t' : (substituteT X U T).
     
 Definition P_Binding (b : Binding) : Prop :=
-  forall Delta Gamma Gamma' X U c c',
-    UpdateContext X U c c' ->
-    Gamma = mupdate empty c ->
-    Gamma' = mupdate empty c' ->
-    forall K b',
-      (X |K-> K; (Delta, Gamma)) |-ok b ->
-      empty |-* U : K ->
-      substituteA_binding X U b b' ->
-      (Delta, Gamma') |-ok b'.
-
+  forall Delta Gamma X K U b',
+    (X |K-> K; (Delta, Gamma)) |-ok b ->
+    empty |-* U : K ->
+    substituteA_binding X U b b' ->
+    (Delta, upd X U Gamma) |-ok b'.
 
 Theorem substituteA_preserves_typing : 
   forall t, P_Term t.
 Proof.
   apply Term__ind with P_Binding.
-  (*- apply skip.
+  - apply skip.
   - (* Var *)
     intros x. 
     unfold P_Term. 
-    intros Delta Gamma X K U T t' c c' Gamma' T'. 
-    intros UC Heq Heq' Htyp Hkind Hsa__t' Hstca__T'.
-
-    assert (forall x, (mupdate empty c) x = lookup x c). {
-      intros. erewrite mupdate_lookup. auto.
-    }
+    intros Delta Gamma X K U T t' Htyp Hkind Hsa__t'.
 
     inversion Htyp. subst.
     inversion Hsa__t'. subst.
 
-    simpl in H2.
-    rewrite H in H2.
-
-    destruct (UpdateContext_domains_match _ _ _ _ UC _ _ H2) as [T0' Hlu__T'].
-
-    apply T_Var.
-    + simpl. rewrite <- mupdate_lookup. assumption. apply Hlu__T'. apply UpdateContext_substituteTCA.
-
-    eapply UpdateContext_domains_match in UC.
-    + apply T_Var.
-      simpl.
-        simpl in H2.
-        apply UC.
-      apply H2.
-
     apply T_Var.
     simpl in H1.
     simpl.
-    apply skip.
     apply upd__substituteT.
     assumption.
   - (* TyAbs*) 
@@ -201,12 +137,14 @@ Proof.
     simpl.
     apply T_LamAbs.
     + unfold P_Term in IH__t_body.
+      unfold extendT.
+      simpl.
       rewrite upd_absorbs_substituteT.
       eapply IH__t_body; eauto.
       unfold extendT in H4.
       simpl in H4.
       apply H4.
-    + simpl. 
+    + simpl.
       eapply substituteT_preserves_kinding.
       * eapply H5.
       * assumption.
@@ -229,6 +167,7 @@ Proof.
     inversion Htyp. subst.
     inversion Hsa__t'. subst.
 
+    simpl.
     eauto with typing.
   - (* Builtin *)
     intros d.
@@ -251,21 +190,25 @@ Proof.
     inversion Htyp. subst.
     inversion Hsa__t'. subst.
 
-    assert ((Delta, UpdateContext X U Gamma) |-+ t0' : (substituteT X U (Ty_Forall X0 K2 T1))) by eauto.
+    assert ((Delta, upd X U Gamma) |-+ t0' : (substituteT X U (Ty_Forall X0 K2 T1))) by eauto.
     
     simpl in H.
     destruct (X =? X0) eqn:Heqb.
-    + eapply T_TyInst.
+    + apply eqb_eq in Heqb. subst.
+      eapply T_TyInst.
       * apply H.
       * eapply substituteT_preserves_kinding; eauto.
-        simpl in H3.
-        apply H3.
+        simpl in H2.
+        simpl.
+        apply H2.
       * apply skip. (* TODO *)
+      * apply skip.
     + eapply T_TyInst.
       * apply H.
       * eapply substituteT_preserves_kinding; eauto.
-        simpl in H3.
-        apply H3.
+        simpl in H2.
+        apply H2.
+      * apply skip.
       * apply skip. (* TODO *)
   - (* Error *)
     intros T0.
@@ -288,8 +231,8 @@ Proof.
 
     simpl.
     eapply T_IWrap.
+    + apply skip. (* TODO *)
     + eauto.
-    + apply skip. (* TODO *) 
     + eapply substituteT_preserves_kinding; eauto.
       apply H6.
     + eapply substituteT_preserves_kinding; eauto.
@@ -300,6 +243,5 @@ Proof.
     intros Delta Gamma X L U T t' Htyp Hkind Hsa__t'.
     
     inversion Htyp. subst.
-    inversion Hsa__t'. subst.*)
-
+    inversion Hsa__t'. subst.
 Admitted.
