src/Language/PlutusIR/Semantics/SemanticEquivalence/CompatibilityLemmas.v
@@ -1,5 +1,6 @@
 (*Require Export PlutusCert.Language.PlutusIR.Semantics.SemanticEquivalence.CompatibilityLemmas.Apply.*)
 Require Export PlutusCert.Language.PlutusIR.Semantics.SemanticEquivalence.CompatibilityLemmas.Constant.
-(*Require Export PlutusCert.Language.PlutusIR.Semantics.SemanticEquivalence.CompatibilityLemmas.IWrap.
-Require Export PlutusCert.Language.PlutusIR.Semantics.SemanticEquivalence.CompatibilityLemmas.Unwrap.*)
+(*Require Export PlutusCert.Language.PlutusIR.Semantics.SemanticEquivalence.CompatibilityLemmas.IWrap.*)
+Require Export PlutusCert.Language.PlutusIR.Semantics.SemanticEquivalence.CompatibilityLemmas.LamAbs.
+(*Require Export PlutusCert.Language.PlutusIR.Semantics.SemanticEquivalence.CompatibilityLemmas.Unwrap.*)
 Require Export PlutusCert.Language.PlutusIR.Semantics.SemanticEquivalence.CompatibilityLemmas.Var.
