src/Language/PlutusIR/Semantics/Static/TypeSubstitution/Equivalence.v
@@ -1,0 +1,12 @@
+Require Import PlutusCert.Language.PlutusIR. 
+Import NamedTerm.
+Require Import PlutusCert.Language.PlutusIR.Semantics.Static.Theorems.ContextInvariance.AFI.
+Require Import PlutusCert.Language.PlutusIR.Semantics.Static.TypeSubstitution.
+Require Import PlutusCert.Language.PlutusIR.Semantics.Static.TypeSubstitution.CaptureAvoiding.
+
+
+Lemma equiv__substituteT__substituteTCA : forall a U T T',
+    closed_Ty U ->
+    substituteTCA a U T T' ->
+    T' = substituteT a U T.
+Proof. Admitted.
