src/Language/PlutusIR/Semantics/TypeSafety/NormalisationPreservesKinding.v
@@ -1,0 +1,22 @@
+Require Import PlutusCert.Language.PlutusIR.
+Import NamedTerm.
+Require Import PlutusCert.Language.PlutusIR.Semantics.Static.
+Require Import PlutusCert.Language.PlutusIR.Semantics.TypeSafety.SubstitutionPreservesTyping.SubstituteTCA.
+
+
+Lemma normalisation_preserves_kinding : forall Delta T T' K,
+    Delta |-* T : K ->
+    normalise T T' ->
+    Delta |-* T' : K.
+Proof.
+  intros.
+  generalize dependent T'.
+  induction H; intros T' Hnorm; try solve [inversion Hnorm; subst; eauto with typing].
+  - inversion Hnorm.
+    + subst.
+      inversion H. subst.
+      eapply substituteTCA_preserves_kinding; eauto.
+      apply skip. (* TODO *)
+    + subst.
+      eauto with typing.
+Qed.
